proof/agp32SpecialScript.sml
@@ -1,0 +1,257 @@
+open hardwarePreamble translatorTheory translatorLib arithmeticTheory wordsExtraTheory dep_rewrite blastLib bitstringSyntax fcpSyntax listSyntax wordsSyntax agp32StateTheory agp32EnvironmentTheory agp32ProcessorTheory ag32Theory ag32ExtraTheory ag32UtilitiesTheory agp32RelationTheory agp32UpdateTheory agp32InternalTheory agp32_EX_CorrectTheory;
+
+(* correctness of special invariants *)
+val _ = new_theory "agp32Special";
+
+val _ = prefer_num ();
+val _ = guess_lengths ();
+
+
+(** when ID and EX are not jump, IF is not NONE **)
+Theorem IF_instr_index_not_none:
+  !I t fext fbits a.
+    is_sch I (agp32 fext fbits) a ==>
+    Rel I (fext t) (agp32 fext fbits (t-1)) (agp32 fext fbits t) a t ==>
+    ~isJump_hw_op (agp32 fext fbits (SUC t)) ==>
+    ~isJump_isa_op (I (2,SUC t)) a ==>
+    I (1,SUC t) <> NONE
+Proof
+  rw [] >> Cases_on `enable_stg 1 (agp32 fext fbits t)` >-
+   (Cases_on `isJump_hw_op (agp32 fext fbits t)` >-
+     fs [is_sch_def,is_sch_fetch_def] >>
+    Cases_on `isJump_isa_op (I' (1,t)) a` >-
+     (`enable_stg 2 (agp32 fext fbits t)`
+        by fs [enable_stg_def,agp32_IF_PC_write_enable_and_ID_ID_write_enable] >>
+      `~isJump_isa_op (I' (2,t)) a` by METIS_TAC [IF_instr_isJump_ID_instr_not_isJump] >>
+      `I' (2,SUC t) = I' (1,t)` by fs [is_sch_def,is_sch_decode_def] >> fs []) >>
+    Cases_on `isJump_isa_op (I' (2,t)) a` >-
+     (`enable_stg 3 (agp32 fext fbits t)`
+        by fs [enable_stg_def,agp32_IF_PC_write_enable_and_ID_EX_write_enable] >>
+      `~reg_data_hazard (agp32 fext fbits t)`
+        by fs [enable_stg_def,isJump_hw_op_def,
+               agp32_IF_PC_write_enable_EX_jump_sel_then_no_reg_data_hazard] >>
+      `I' (3,SUC t) = I' (2,t)` by fs [is_sch_def,is_sch_execute_def] >>
+      `isJump_isa_op (I' (3,SUC t)) a` by fs [] >>
+      cheat) >>
+    Cases_on `I' (1,t) = NONE` >> fs [] >>
+    fs [is_sch_def,is_sch_fetch_def] >>
+    fs [Rel_def,Inv_Rel_def]) >>
+  `~enable_stg 2 (agp32 fext fbits t)`
+    by METIS_TAC [enable_stg_def,agp32_IF_PC_write_enable_and_ID_ID_write_enable] >>  
+  fs [is_sch_def,is_sch_disable_def] >>
+  Cases_on `enable_stg 3 (agp32 fext fbits t)` >-
+   (Cases_on `isJump_hw_op (agp32 fext fbits t)` >> fs [] >-
+     METIS_TAC [enable_stg_def,agp32_ID_EX_write_enable_isJump_hw_op_IF_PC_write_enable] >>
+    fs [Rel_def,Inv_Rel_def] >> METIS_TAC []) >>
+  `isJump_hw_op (agp32 fext fbits (SUC t)) = isJump_hw_op (agp32 fext fbits t)`
+    by cheat >>
+  fs [Rel_def,Inv_Rel_def] >> METIS_TAC []
+QED
+
+(** Jump in the EX stage under special ID conditions  **)
+Theorem ID_NONE_exists_a_jump:
+  !I fext fbits a t.
+    is_sch I (agp32 fext fbits) a ==>
+    Rel I (fext t) (agp32 fext fbits (t-1)) (agp32 fext fbits t) a t ==>
+    enable_stg 2 (agp32 fext fbits t) ==>
+    ~isJump_hw_op (agp32 fext fbits (SUC t)) ==>
+    I (2,SUC t) = NONE ==>
+    isJump_hw_op (agp32 fext fbits t)
+Proof
+  rw [is_sch_def] >>
+  Cases_on `isJump_hw_op (agp32 fext fbits t)` >> fs [] >>
+  Cases_on `isJump_isa_op (I' (2,t)) a` >-
+   (`enable_stg 3 (agp32 fext fbits t)`
+      by fs [enable_stg_def,agp32_ID_ID_write_enable_and_ID_EX_write_enable] >>
+    `~reg_data_hazard (agp32 fext fbits t)`
+      by fs [enable_stg_def,isJump_hw_op_def,
+             agp32_ID_ID_write_enable_EX_jump_sel_then_no_reg_data_hazard] >>
+    `I' (3,SUC t) = I' (2,t)` by fs [is_sch_execute_def] >> rw [] >>
+    `isJump_isa_op (I' (3,SUC t)) a` by fs [] >>
+    cheat) >>
+  `I' (2,SUC t) = I' (1,t)` by METIS_TAC [is_sch_decode_def] >> fs [] >>
+  Cases_on `t` >> fs [] >-
+   fs [enable_stg_def,agp32_init_ctrl_flags] >>
+  fs [Rel_def,Inv_Rel_def]
+QED
+
+(** there exists a jump at t-1 when I (3,SUC t) = I (2,t) = NONE **)
+Theorem EX_NONE_previous_jump_special:
+  !I fext fbits a t.
+    is_sch I (agp32 fext fbits) a ==>
+    Rel I (fext t) (agp32 fext fbits (t-1)) (agp32 fext fbits t) a t ==>
+    enable_stg 2 (agp32 fext fbits t) ==>
+    enable_stg 3 (agp32 fext fbits (SUC t)) ==>
+    ~isJump_hw_op (agp32 fext fbits (SUC t)) ==>
+    ~reg_data_hazard (agp32 fext fbits (SUC t)) ==>
+    I (3,SUC (SUC t)) = NONE ==>
+    isJump_hw_op (agp32 fext fbits t)
+Proof
+  rw [] >>
+  `I' (3,SUC (SUC t)) = I' (2,SUC t)` by METIS_TAC [is_sch_def,is_sch_execute_def] >>
+  METIS_TAC [ID_NONE_exists_a_jump]
+QED
+
+(** ID_opc is 15 under certain conditions **)
+Theorem ID_instr_index_NONE_opc_flush_when_disabled:
+  !I t fext fbits a.
+    is_sch I (agp32 fext fbits) a ==>
+    Rel I (fext t) (agp32 fext fbits (t-1)) (agp32 fext fbits t) a t ==>
+    ~enable_stg 2 (agp32 fext fbits t) ==>
+    ~isJump_hw_op (agp32 fext fbits (SUC t)) ==>
+    I (2,SUC t) = NONE ==>
+    (agp32 fext fbits (SUC t)).ID.ID_opc = 15w
+Proof
+  rw [] >> `I' (2,SUC t) = I' (2,t)` by METIS_TAC [is_sch_def,is_sch_disable_def] >>
+  `(agp32 fext fbits (SUC t)).ID.ID_opc = (agp32 fext fbits t).ID.ID_opc`
+    by fs [ID_opc_unchanged_when_ID_disabled] >>
+  Cases_on `enable_stg 2 (agp32 fext fbits (t-1))` >-
+   (Cases_on `~isJump_hw_op (agp32 fext fbits t)` >> fs [] >-
+     (`isJump_hw_op (agp32 fext fbits (t − 1))` by fs [Rel_def,Inv_Rel_def] >>
+      `(agp32 fext fbits (SUC (t-1))).ID.ID_opc = 15w` by fs [EX_isJump_hw_op_next_ID_opc] >>
+      Cases_on `t` >> fs []) >>
+    Cases_on `~enable_stg 3 (agp32 fext fbits t)` >-
+     (`isJump_hw_op (agp32 fext fbits (SUC t)) = isJump_hw_op (agp32 fext fbits t)`
+        by cheat >> fs []) >>
+    fs [enable_stg_def] >>
+    METIS_TAC [agp32_IF_PC_write_enable_and_ID_ID_write_enable,
+               agp32_ID_EX_write_enable_isJump_hw_op_IF_PC_write_enable]) >>
+  fs [] >> Cases_on `~isJump_hw_op (agp32 fext fbits t)` >> fs [] >-
+   fs [Rel_def,Inv_Rel_def] >>
+  Cases_on `~enable_stg 3 (agp32 fext fbits t)` >-
+   (`isJump_hw_op (agp32 fext fbits (SUC t)) = isJump_hw_op (agp32 fext fbits t)`
+      by cheat >> fs []) >>
+  fs [enable_stg_def] >>
+  METIS_TAC [agp32_IF_PC_write_enable_and_ID_ID_write_enable,
+             agp32_ID_EX_write_enable_isJump_hw_op_IF_PC_write_enable]
+QED
+
+(** EX_opc is flushed **)
+Theorem EX_instr_index_NONE_opc_flush:
+  !I t fext fbits a.
+    is_sch I (agp32 fext fbits) a ==>
+    Rel I (fext t) (agp32 fext fbits (t-1)) (agp32 fext fbits t) a t ==>
+    I (3,SUC t) = NONE ==>
+    ((agp32 fext fbits (SUC t)).EX.EX_opc = 16w) \/ ((agp32 fext fbits (SUC t)).EX.EX_opc = 15w)
+Proof
+  rw [] >> Cases_on `enable_stg 3 (agp32 fext fbits t)` >-
+   (Cases_on `isJump_hw_op (agp32 fext fbits t)` >-
+     (`(agp32 fext fbits t).EX.EX_NOP_flag`
+        by fs [enable_stg_def,agp32_ID_EX_write_enable_isJump_hw_op_EX_NOP_flag] >>
+      fs [agp32_EX_opc_flush_when_EX_NOP_flag]) >>
+    Cases_on `reg_data_hazard (agp32 fext fbits t)` >-
+     (`(agp32 fext fbits t).EX.EX_NOP_flag`
+        by fs [enable_stg_def,agp32_ID_EX_write_enable_reg_data_hazard_EX_NOP_flag] >>
+      fs [agp32_EX_opc_flush_when_EX_NOP_flag]) >>
+    `I' (3,SUC t) = I' (2,t)` by METIS_TAC [is_sch_def,is_sch_execute_def] >> fs [] >>
+    `~(agp32 fext fbits t).EX.EX_NOP_flag`
+      by fs [enable_stg_def,agp32_ID_EX_write_enable_no_jump_or_reg_data_hazard_EX_NOP_flag_F] >>
+    `(agp32 fext fbits (SUC t)).EX.EX_opc = (agp32 fext fbits t).ID.ID_opc`
+      by fs [agp32_EX_opc_ID_opc_when_not_EX_NOP_flag] >> fs [] >>
+    Cases_on `enable_stg 2 (agp32 fext fbits (t-1))` >-
+     (`isJump_hw_op (agp32 fext fbits (t-1))` by fs [Rel_def,Inv_Rel_def] >>
+      `(agp32 fext fbits (SUC (t-1))).ID.ID_opc = 15w` by fs [EX_isJump_hw_op_next_ID_opc] >>
+      Cases_on `t` >> fs []) >>
+    fs [Rel_def,Inv_Rel_def]) >>
+  `I' (3,SUC t) = I' (3,t)` by METIS_TAC [is_sch_def,is_sch_disable_def] >>
+  fs [agp32_EX_opc_unchanged_when_EX_disabled,Rel_def,Inv_Rel_def]
+QED
+
+(** EX_write_reg **)
+Theorem EX_instr_index_NONE_EX_not_write_reg:
+  !I t fext fbits a.
+    is_sch I (agp32 fext fbits) a ==>
+    Rel I (fext t) (agp32 fext fbits (t-1)) (agp32 fext fbits t) a t ==>
+    I (3,SUC t) = NONE ==>
+    ~(agp32 fext fbits (SUC t)).EX.EX_write_reg
+Proof
+  rw [is_sch_def] >>
+  Cases_on `enable_stg 3 (agp32 fext fbits t)` >-
+   (Cases_on `isJump_hw_op (agp32 fext fbits t)` >-
+     (`(agp32 fext fbits t).EX.EX_NOP_flag`
+        by fs [enable_stg_def,agp32_ID_EX_write_enable_isJump_hw_op_EX_NOP_flag] >>
+      fs [agp32_EX_write_reg_F_when_EX_NOP_flag]) >>
+    Cases_on `reg_data_hazard (agp32 fext fbits t)` >-
+     (`(agp32 fext fbits t).EX.EX_NOP_flag`
+        by fs [enable_stg_def,agp32_ID_EX_write_enable_reg_data_hazard_EX_NOP_flag] >>
+      fs [agp32_EX_write_reg_F_when_EX_NOP_flag]) >>
+    `((agp32 fext fbits (SUC t)).EX.EX_opc = 16w) \/ ((agp32 fext fbits (SUC t)).EX.EX_opc = 15w)`
+      by METIS_TAC [is_sch_def,EX_instr_index_NONE_opc_flush] >>
+    `~(agp32 fext fbits t).EX.EX_NOP_flag`
+      by fs [enable_stg_def,agp32_ID_EX_write_enable_no_jump_or_reg_data_hazard_EX_NOP_flag_F] >>
+    fs [agp32_EX_write_reg_F_when_EX_opc_flushed]) >>
+  `I' (3,SUC t) = I' (3,t)` by METIS_TAC [is_sch_disable_def] >>
+  fs [agp32_EX_write_reg_unchanged_when_EX_disabled,Rel_def,Inv_Rel_def]
+QED
+
+(** instr index relation between IF and WB stages when ID, EX and MEM are NONE **)
+Theorem IF_instr_index_with_WB_instr_ID_EX_MEM_NONE:
+  !I t fext fbits a.
+    is_sch I (agp32 fext fbits) a ==>
+    Rel I (fext t) (agp32 fext fbits (t-1)) (agp32 fext fbits t) a t ==>
+    I (1,SUC t) <> NONE ==>
+    I (2,SUC t) = NONE ==>
+    I (3,SUC t) = NONE ==>
+    I (4,SUC t) = NONE ==>
+    I (5,SUC t) <> NONE ==>
+    (THE (I (1,SUC t)) > THE (I (5,SUC t))) /\ (THE (I (1,SUC t)) < THE (I (5,SUC t)) + 2)
+Proof
+  rpt gen_tac >> rpt disch_tac >>
+  Cases_on `enable_stg 1 (agp32 fext fbits t)` >-
+   (Cases_on `isJump_hw_op (agp32 fext fbits t)` >-
+     (`I' (1,SUC t) = SOME (THE (I' (3,t)) + 1)` by fs [is_sch_def,is_sch_fetch_def] >>
+      `isJump_isa_op (I' (3,t)) a` by fs [Rel_def,EX_Rel_spec_def,isJump_hw_op_def] >>
+      `I' (3,t) <> NONE` by METIS_TAC [isJump_isa_op_not_none] >>
+      `enable_stg 4 (agp32 fext fbits t)`
+        by fs [enable_stg_def,agp32_IF_PC_write_enable_and_MEM_flag] >>
+      `enable_stg 3 (agp32 fext fbits t)`
+        by fs [enable_stg_def,agp32_IF_PC_write_enable_and_ID_EX_write_enable] >>
+      Cases_on `isMemOp_hw_op (agp32 fext fbits t)` >-
+       (fs [enable_stg_def] >>
+        METIS_TAC [MEM_stg_op_agp32_ID_EX_write_disable]) >>
+      `I' (4,SUC t) = I' (3,t)` by METIS_TAC [is_sch_def,is_sch_memory_def] >> fs []) >>
+    Cases_on `isJump_isa_op (I' (1,t)) a \/ isJump_isa_op (I' (2,t)) a \/ I' (1,t) = NONE` >-
+     (fs [is_sch_def,is_sch_fetch_def,is_sch_execute_def] >> METIS_TAC []) >> fs [] >>
+    `enable_stg 2 (agp32 fext fbits t)`
+      by fs [enable_stg_def,agp32_IF_PC_write_enable_and_ID_ID_write_enable] >>
+    `I' (2,SUC t) = I' (1,t)` by METIS_TAC [is_sch_def,is_sch_decode_def] >> fs []) >>
+  `~enable_stg 2 (agp32 fext fbits t)`
+    by METIS_TAC [enable_stg_def,agp32_IF_PC_write_enable_and_ID_ID_write_enable] >>
+  Cases_on `enable_stg 5 (agp32 fext fbits t)` >-
+   (`I' (5,SUC t) = I' (4,t)` by fs [is_sch_def,is_sch_writeback_def] >>
+    Cases_on `~enable_stg 3 (agp32 fext fbits t)` >> fs [] >-
+     (`I' (1,SUC t) = I' (1,t) /\ I' (2,SUC t) = I' (2,t) /\ I' (3,SUC t) = I' (3,t)`
+        by METIS_TAC [is_sch_def,is_sch_disable_def] >> fs [] >>
+      METIS_TAC [IF_instr_index_with_MEM_instr_ID_EX_NONE]) >>
+    `enable_stg 4 (agp32 fext fbits t)`
+      by fs [enable_stg_def,agp32_MEM_state_flag_eq_WB_state_flag] >>
+    `~isMemOp_hw_op (agp32 fext fbits t)`
+      by fs [enable_stg_def,agp32_ID_EX_write_enable_no_MEM_stg_op] >>
+    `I' (4,SUC t) = I' (3,t)` by METIS_TAC [is_sch_def,is_sch_memory_def] >> fs [] >>
+    `I' (1,SUC t) = I' (1,t) /\ I' (2,SUC t) = I' (2,t)`
+      by METIS_TAC [is_sch_def,is_sch_disable_def] >> fs [] >>
+    METIS_TAC [IF_instr_index_with_MEM_instr_ID_EX_NONE]) >>
+  `~enable_stg 4 (agp32 fext fbits t)` by fs [enable_stg_def,agp32_MEM_state_flag_eq_WB_state_flag] >>
+  `~enable_stg 3 (agp32 fext fbits t)`
+    by fs [enable_stg_def,agp32_MEM_state_flag_F_and_ID_EX_write_disable] >>
+  `I' (1,SUC t) = I' (1,t) /\ I' (2,SUC t) = I' (2,t) /\ I' (3,SUC t) = I' (3,t) /\
+  I' (4,SUC t) = I' (4,t) /\ I' (5,SUC t) = I' (5,t)`
+    by METIS_TAC [is_sch_def,is_sch_disable_def] >>
+  fs [Rel_def,Inv_Rel_def]
+QED
+
+
+(* Inv_Rel *)
+Theorem agp32_Rel_ag32_Inv_Rel_correct:
+  !fext fbits a t I.
+    is_sch I (agp32 fext fbits) a ==>
+    Rel I (fext t) (agp32 fext fbits (t-1)) (agp32 fext fbits t) a t ==>
+    Inv_Rel I (agp32 fext fbits t) (agp32 fext fbits (SUC t)) a (SUC t)
+Proof
+  rw [Inv_Rel_def] >>
+  METIS_TAC [IF_instr_index_not_none,ID_NONE_exists_a_jump,EX_NONE_previous_jump_special,
+             ID_instr_index_NONE_opc_flush_when_disabled,EX_instr_index_NONE_opc_flush,
+             EX_instr_index_NONE_EX_not_write_reg,IF_instr_index_with_WB_instr_ID_EX_MEM_NONE]
+QED
+
+val _ = export_theory ();
